stdlib/iterator/theories/map.v
@@ -77,6 +77,48 @@ Global Hint Extern 100 (SimplExist (map_inv_ty _ _ _ _ ?fnonce) _ _) =>
   notypeclasses refine (simpl_exist_map_inv_pure_pre _ _ _ _ fnonce _ _);
   typeclasses eauto : typeclass_instances.
 
+(** Instantiation hints for iterator adapters which receive a closure param instantiation predicate *)
+Section clos_param_variants.
+  Context `{!refinedrustGS Σ}.
+
+  Definition clos_param_pred_ty (Args_rt Clos_rt Clos_out_rt : RT)
+    (fnonce_attrs : FnOnce_spec_attrs Clos_rt Args_rt Clos_out_rt) :=
+    fnonce_attrs.(FnOnce_Params) → Prop.
+  Global Arguments clos_param_pred_ty : simpl never.
+
+  Context (Args_rt Clos_rt Clos_out_rt : RT)
+    (fnonce_attrs : FnOnce_spec_attrs Clos_rt Args_rt Clos_out_rt).
+
+  (* Default instantiation *)
+  Lemma simpl_exist_clos_param_pred_trivial Q :
+    SimplExist (clos_param_pred_ty _ _ _ fnonce_attrs) Q
+      (∃ (ParamPred : fnonce_attrs.(FnOnce_Params) → Prop), Q ParamPred).
+  Proof. unfold SimplExist. done. Qed.
+  Lemma simpl_forall_clos_param_pred Q :
+    SimplForall (clos_param_pred_ty _ _ _ fnonce_attrs) 1 Q (∀ (ParamPred : fnonce_attrs.(FnOnce_Params) → Prop), Q ParamPred).
+  Proof. unfold SimplForall. done. Qed.
+
+  (* For trivial Params, instantiate with a trivial invariant *)
+  Lemma simpl_exist_clos_param_pred_empty Q :
+    TCDone (fnonce_attrs.(FnOnce_Params) = plist id []) →
+    SimplExist (clos_param_pred_ty Args_rt Clos_rt Clos_out_rt fnonce_attrs) Q
+      (Q (λ _, True)).
+  Proof.
+    intros Hpre.
+    unfold SimplExist.
+    eauto with iFrame.
+  Qed.
+End clos_param_variants.
+Global Hint Extern 1000 (SimplExist (clos_param_pred_ty _ _ _ ?fnonce) _ _) =>
+  notypeclasses refine (simpl_exist_clos_param_pred_trivial _ _ _ fnonce _) : typeclass_instances.
+Global Hint Extern 10 (SimplForall (clos_param_pred_ty _ _ _ ?fnonce) _ _ _) =>
+  notypeclasses refine (simpl_forall_clos_param_pred _ _ _ fnonce _) : typeclass_instances.
+
+Global Hint Extern 100 (SimplExist (clos_param_pred_ty _ _ _ ?fnonce) _ _) =>
+  notypeclasses refine (simpl_exist_clos_param_pred_empty _ _ _ fnonce _ _);
+  typeclasses eauto : typeclass_instances.
+
+
 Section map.
   Context `{RRGS : !refinedrustGS Σ}.
   Definition MapInv {Self_rt Item_rt Clos_rt Clos_out_rt : RT} {ClosParams : Type}
@@ -84,7 +126,8 @@ Section map.
     (Pre : thread_id → ClosParams → RT_xt Clos_rt → RT_xt (tuple1_rt Item_rt) → iProp Σ)
     (PostMut : thread_id → ClosParams → RT_xt Clos_rt → RT_xt (tuple1_rt Item_rt) → RT_xt Clos_rt → RT_xt Clos_out_rt → iProp Σ)
     : _ → _ → _ → iProp Σ :=
-    λ (π : thread_id) (inner_p : _) (s : MapX Self_rt Clos_rt),
+    λ (π : thread_id) (p : _ * (ClosParams → Prop)) (s : MapX Self_rt Clos_rt),
+    let '(inner_p, ParamPred) := p in
     (∃ (Inv : thread_id → RT_xt Self_rt → RT_xt Clos_rt → iProp Σ),
       (* user-picked invariant *)
       Inv π s.(map_it) s.(map_clos) ∗
@@ -94,8 +137,8 @@ Section map.
       li_sealed (□ (∀ it_state it_state' clos_state e,
         (☒ iter_attrs.(traits_iterator_Iterator_Next) π inner_p it_state (Some e) it_state') -∗
         Inv π it_state clos_state -∗
-        ∃ p, Pre π p clos_state *[e] ∗
-        (∀ e' clos_state', ☒ PostMut π p clos_state *[e] clos_state' e' -∗ Inv π it_state' clos_state'))) ∗
+        ∃ p_clos, ⌜ParamPred p_clos⌝ ∗ Pre π p_clos clos_state *[e] ∗
+        (∀ e' clos_state', ☒ PostMut π p_clos clos_state *[e] clos_state' e' -∗ Inv π it_state' clos_state'))) ∗
       (* progress (no element) *)
       li_sealed (□ (∀ it_state it_state' clos_state,
         (☒ iter_attrs.(traits_iterator_Iterator_Next) π inner_p it_state None it_state') -∗
